\documentclass[11pt]{article} 

% packages with special commands
\usepackage{amssymb, amsmath}
\usepackage{epsfig}
\usepackage{array}
\usepackage{ifthen}
\usepackage{color}
%\usepackage{fancyhdr}
\usepackage{graphicx}
\usepackage{indentfirst}
\usepackage{caption}
%\usepackage{mathtools}
\definecolor{grey}{rgb}{0.5,0.5,0.5}

\begin{document}
\newcommand{\tr}{\text{tr}}
\newcommand{\E}{\textbf{E}}
\newcommand{\diag}{\text{diag}}
\newcommand{\argmax}{\text{argmax}}
\newcommand{\argmin}{\text{argmin}}
\newcommand{\Cov}{\text{Cov}}
\newcommand{\Vol}{\text{Vol}}
%\pagestyle{fancy}

\title{Notes on Information Geometry}

\author{Charles Zheng}


\maketitle



\section{Definitions}

The $\alpha$-connection
\[
\Gamma^{(\alpha)}_{ij, k}(\theta) = \E_\theta[((\partial_i\partial_j \ell_\theta) - (\partial_i \ell_\theta)(\partial_j \ell_\theta)) \partial_k \ell_\theta]
\]

\section{Exponential families}       

\subsection{Definitions}
\[
p_\theta(x) = C(x) \exp[\Sigma_i \theta_i t_i(x) - \psi(\theta)]
\]
\[
\ell_\theta(x) = \log p_\theta(x) = \log C(x) + \sum_i \theta_i t_i(x) - \psi(\theta)
\]
\[
\psi(\theta) = \log \int_x C(x) e^{\theta^T t(x)} dx
\]
\[
\eta_i(\theta) = \E_\theta[t_i(X)]
\]
\[
g_{ij}(\theta) = \Cov_\theta[t_i(X), t_j(X)] = g_{ji}
\]

\subsection{Properties under natural parameterization}
\[
\partial_i \stackrel{\Delta}{=} \frac{\partial}{\partial \theta_i}
\]
\[
\partial_i \psi(\theta) = \eta_i(\theta)
\]
\[
\partial_i \partial_j \psi(\theta) = g_{ij}(\theta)
\]
\[
\partial_i \ell(x) = t_i(x) - \eta_i
\]
Note that $\partial_i \partial_j \ell(x)$ is constant as a function of $x$.
\[
\partial_i \partial_j \ell(x) = -g_{ij}
\]
\[
\partial_i \partial_j \partial_k \ell(x) = -\partial_k g_{ij} = -\mathbb{E}(\partial_i \ell)(\partial_j \ell)(\partial_k \ell) \stackrel{D}{=} - T_{ijk}
\]
\[
T_{ijk} = \partial_k g_{ij}  = T_{ikj} = \cdots = T_{kji}
\]

\subsection{Natural parameterization is e-affine}

\[
\Gamma^{(1)}_{ij, k}(\theta) = \E_\theta[(\partial_i \partial_j \ell)(\partial_k \ell)] = -g_{ij} \E[\partial_k \ell] = 0
\]

\subsection{Properties under mean ($\eta$) parameterization}


\[
\frac{\partial \eta_i}{\partial \theta_j} = \partial_j (\partial_i \psi) = g_{ij}
\]
\[
\tilde{\partial}_i \stackrel{\Delta}{=} \frac{\partial}{\partial \eta_i} = \sum_j \frac{\partial \theta_j}{\partial \eta_i} \partial_j = \sum_j \frac{\partial_j}{g_{ij}}
\]

\subsubsection{Properties of $T_{ijk}$}

We have
\[
\frac{\partial^2 \theta_k}{\partial \eta_i \partial \eta_j} = \tilde{\partial}_j \frac{1}{g_{ik}} = \tilde{\partial}_i \frac{1}{g_{jk}}
\]
therefore
\[
\sum_m \frac{1}{g_{jm}} \frac{T_{ikm}}{g_{ik}^2} = \sum_m \frac{1}{g_{im}} \frac{T_{jkm}}{g_{jk}^2}
\]
Hence, if we define
\[
C_{ijk} \stackrel{\Delta}{=} \frac{1}{g_{ik}^2} \sum_m \frac{T_{ikm}}{g_{jm}} = -\frac{\partial^2 \theta_k}{\partial \eta_i \partial \eta_j}
\]
then we have
\[
C_{ijk} = C_{jik}
\]
by definition, and from symmetry of $T_{ijk}$ we have
\[
C_{ijk} = C_{kji}
\]
hence $C_{ijk} = C_{kji} = C_{jki} = \cdots$, i.e. is symmetric with respect to indices.

\subsubsection{Derivatives}

\[
\tilde{\partial}_i \ell = \sum_k \frac{\partial_k \ell}{g_{ik}}
\]
\[
\tilde{\partial}_i \tilde{\partial}_j \ell = -\left(\sum_k C_{ijk} \partial_k \ell \right) - \left(\sum_{k,m} \frac{g_{km}}{g_{ik}g_{jm}}\right)
\]

\subsubsection{Mean parameterization is m-affine}

\begin{align*}
\Gamma^{(-1)}_{ij,k}(\eta) &= \E_\eta[(\tilde{\partial}_i\tilde{\partial}_j \ell) (\tilde{\partial}_k \ell) 
+ (\tilde{\partial}_i \ell)(\tilde{\partial}_j \ell)(\tilde{\partial}_k \ell)]
\\&= \E\left[\left(-\left(\sum_k C_{ijk} \partial_k \ell  + \sum_{k,m} \frac{g_{km}}{g_{ik}g_{jm}}\right) + (\tilde{\partial}_i \ell)(\tilde{\partial}_j \ell)\right)(\tilde{\partial_k} \ell)\right]
\end{align*}

\begin{align*}
\E[(\tilde{\partial}_i \ell)(\tilde{\partial}_j \ell)(\tilde{\partial}_k \ell)] 
&= \sum_{a,b,c} \frac{\E[(\partial_a \ell)(\partial_b \ell)(\partial_c \ell)]}{g_{ia}g_{jb}g_{kc}}
\\&= \sum_{a,b,c} \frac{T_{abc}}{g_{ia}g_{jb}g_{kc}}
\end{align*}

\begin{align*}
\E_\eta[(\tilde{\partial}_i\tilde{\partial}_j \ell) (\tilde{\partial}_k \ell)]  &= 
\E\left[\left(-\sum_k C_{ijk} \partial_k \ell  - \sum_{k,m} \frac{g_{km}}{g_{ik}g_{jm}}\right)(\tilde{\partial}_k \ell)\right]
\\&= - \E\left[   \left(\sum_a C_{ija} \partial_a \ell\right) \left(\sum_{b} \frac{\partial_b \ell}{g_{kb}}\right)\right]
\\&= -\sum_{a, b} \frac{C_{ija}}{g_{kb}} \E[(\partial_a \ell)(\partial_b \ell)] = -\sum_{a,b} \frac{C_{ija} g_{ab}}{g_{kb}}
\end{align*}
\end{document}
